pulse/examples/dsls/mini_steel/Pulse.Soundness.While.fsti
@@ -1,0 +1,39 @@
+module Pulse.Soundness.While
+
+open FStar.Reflection
+open Refl.Typing
+open Pulse.Elaborate.Pure
+open Pulse.Typing
+open Pulse.Soundness.Common
+
+(*
+
+ g |- inv  : bool -> vprop
+ g |- cond : stt<0> bool (exists_ inv) inv
+ g |- body : stt<0> unit (inv true) (fun _ -> exists_ inv)
+ -------------------------------------------------------------------------
+ g |- while inv cond body : stt<0> unit (exists_ inv) (fun _ -> inv false)
+
+*)
+
+val while_soundness
+  (#f:stt_env)
+  (#g:env)
+  (#inv:term)
+  (#cond:term)
+  (#body:term)
+  (inv_typing:typing (extend_env_l f g)
+                     inv
+                     (mk_arrow (bool_tm, Q_Explicit) vprop_tm))
+  (cond_typing:typing (extend_env_l f g)
+                      cond
+                      (mk_stt_comp uzero bool_tm (mk_exists uzero bool_tm inv) inv))
+  (body_typing:typing (extend_env_l f g)
+                      body
+                      (mk_stt_comp uzero unit_tm
+                         (pack_ln (Tv_App inv (true_tm, Q_Explicit)))
+                         (mk_abs unit_tm Q_Explicit (mk_exists uzero bool_tm inv))))
+  : typing (extend_env_l f g)
+           (mk_while inv cond body)
+           (mk_stt_comp uzero unit_tm (mk_exists uzero bool_tm inv)
+              (mk_abs unit_tm Q_Explicit (pack_ln (Tv_App inv (false_tm, Q_Explicit)))))
